Updaets

high2/Zeta.High.Merkle.fst
@@ -1,13 +1,134 @@
 module Zeta.High.Merkle
 
-open Zeta.App
-open Zeta.BinTreePtr
-open Zeta.Interleave
-open Zeta.Merkle
-
 module HV = Zeta.High.Verifier
-module BP=Zeta.BinTreePtr
-module M=Zeta.Merkle
+module BP = Zeta.BinTreePtr
+module M = Zeta.Merkle
+
+let stored_value (#app:_) = HV.stored_value #app
+
+(* three type of edge additions due to AddM (k,_) k' *)
+type addm_t=
+  | NoNewEdge         (* common case: no new added; k' points k *)
+  | NewEdge           (* new edge added: k' points to none along k direction *)
+  | CutEdge           (* cut an existing edge: k' points to k2, is_proper_desc k2 k *)
+
+let addm_props (#app #n:_) (il: eac_log app n) (i: seq_index il{AddM? (index il i)})
+  : Lemma (ensures (let AddM (gk, gv) k k' = index il i in
+                    let il' = prefix il i in
+                    is_proper_desc k k' /\
+                    (let v' = eac_merkle_value k' il' in
+                     let c = desc_dir k k' in
+                     let dh' = desc_hash v' c in
+                     match dh' with
+                     | Empty -> gv = init_value gk
+                     | Desc k2 h2 b2 -> (k2 = k /\ h2 = hashfn gv /\ b2 = false) \/
+                                        (is_proper_desc k2 k /\ gv = init_value gk))))
+          [SMTPat (index il i)]
+  = admit()
+
+let addm_type (#app #n:_) (il: eac_log app n) (i: seq_index il{AddM? (index il i)})
+  : addm_t
+  = let AddM (gk, gv) k k' = index il i in
+    let il' = prefix il i in
+    let v' = eac_merkle_value k' il' in
+    let c = desc_dir k k' in
+    let dh' = desc_hash v' c in
+    match dh' with
+    | Empty -> NewEdge
+    | Desc k2 h2 b2 -> if k2 = k then NoNewEdge else CutEdge
+
+let evictm_props (#app #n:_) (il: eac_log app n) (i: seq_index il{EvictM? (index il i)})
+  : Lemma (ensures (let EvictM k k' = index il i in
+                    let il' = prefix il i in
+                    let esk = eac_state_of_key_pre k il i in
+                    let esk' = eac_state_of_key_pre k' il i in
+                    is_proper_desc k k' /\ EACInStore? esk /\ EACInStore? esk'))
+          [SMTPat (index il i)]
+  = admit()
+
+let evictbm_props (#app #n:_) (il: eac_log app n) (i: seq_index il{EvictBM? (index il i)})
+  : Lemma (ensures (let EvictBM k k' _ = index il i in
+                    let il' = prefix il i in
+                    let esk = eac_state_of_key_pre k il i in
+                    let esk' = eac_state_of_key_pre k' il i in
+                    is_proper_desc k k' /\ EACInStore? esk /\ EACInStore? esk'))
+          [SMTPat (index il i)]
+  = admit()
+
+let only_data_keys_ref_runapp (#app #n:_) (il: eac_log app n) (i: seq_index il{RunApp? (index il i)}) (k: base_key)
+  : Lemma (ensures (let e = index il i in
+                    e `refs_key` k ==> is_leaf_key k))
+  = admit()
+
+let eac_value_init
+  (#app #n:_)
+  (gk: key app)
+  (il: eac_log app n {length il = 0})
+  : Lemma (ensures (eac_value gk il = init_value gk))
+  = admit()
+
+let eac_value_snoc
+  (#app #n:_)
+  (gkf: key app)
+  (il: eac_log app n {length il > 0})
+  : Lemma (ensures (let i = length il - 1 in
+                    let il' = prefix il i in
+                    let e = index il i in
+                    let bkf = to_base_key gkf in
+                    match e with
+                    | AddM (gk,gv) k k' -> (
+                      let c = desc_dir k k' in
+                      match (addm_type il i) with
+                      | NoNewEdge -> eac_value gkf il = eac_value gkf il'
+                      | NewEdge -> if k' = bkf
+                                   then
+                                     let v' = eac_merkle_value k' il' in
+                                     let v' = update_value v' c k Zeta.Hash.zero false in
+                                     eac_value gkf il = IntV v'
+                                   else
+                                     eac_value gkf il = eac_value gkf il'
+                      | CutEdge -> if k = bkf then
+                                     let v = eac_merkle_value k il' in
+                                     let v' = eac_merkle_value k' il' in
+                                     let Desc k2 h2 b2 = desc_hash v' c in
+                                     let c2 = desc_dir k2 k in
+                                     let v = update_value v c2 k2 h2 b2 in
+                                     eac_value gkf il = IntV v
+                                   else if k' = bkf then
+                                     let v' = eac_merkle_value k' il' in
+                                     let v' = update_value v' c k Zeta.Hash.zero false in
+                                     eac_value gkf il = IntV v'
+                                   else
+                                     eac_value gkf il = eac_value gkf il'
+                      )
+                    | AddB _ _ _ _ -> eac_value gkf il = eac_value gkf il'
+                    | EvictM k k' -> if k' = bkf then
+                                       let v' = eac_merkle_value k' il' in
+                                       let gk = to_gen_key k il' in
+                                       let v = eac_value gk il' in
+                                       let c = desc_dir k k' in
+                                       let v' = update_value v' c k (hashfn v) false in
+                                       eac_value gkf il = IntV v'
+                                     else
+                                       eac_value gkf il = eac_value gkf il'
+                    | EvictB _ _ -> eac_value gkf il = eac_value gkf il'
+                    | EvictBM k k' _ -> if k' = bkf then
+                                       let v' = eac_merkle_value k' il' in
+                                       let gk = to_gen_key k il' in
+                                       let v = eac_value gk il' in
+                                       let c = desc_dir k k' in
+                                       let v' = update_value v' c k (hashfn v) false in
+                                       eac_value gkf il = IntV v'
+                                     else
+                                       eac_value gkf il = eac_value gkf il'
+                    | VerifyEpoch -> eac_value gkf il = eac_value gkf il'
+                    | NextEpoch -> eac_value gkf il = eac_value gkf il'
+                    | RunApp _ _ _ -> if e `refs_key` bkf then
+                                        True
+                                      else
+                                       eac_value gkf il = eac_value gkf il'
+  ))
+  = admit()
 
 (* does the log entry update which descendant the value of k points to? *)
 let updates_points_to (#app:_) (e: vlog_entry app) (k: merkle_key): bool =
@@ -15,93 +136,52 @@ let updates_points_to (#app:_) (e: vlog_entry app) (k: merkle_key): bool =
   | AddM r k1 k2 -> k1 = k || k2 = k
   | _ -> false
 
-let is_keyed (#app:_) (e: vlog_entry app)
-  = match e with
-    | AddM _ _ _
-    | AddB _ _ _ _
-    | EvictM _ _
-    | EvictB _ _
-    | EvictBM _ _ _ -> true
-    | _ -> false
-
-let key_of (#app:_) (e: vlog_entry app {is_keyed e})
-  = match e with
-    | AddM _ k _ -> k
-    | AddB _ k _ _ -> k
-    | EvictM k _ -> k
-    | EvictB k _ -> k
-    | EvictBM k _ _ -> k
-
-let ptrfn_aux (#app #n:_) (il: eac_log app n) (k:merkle_key) (c:bin_tree_dir)
+let eac_ptrfn_aux (#app #n:_) (il: eac_log app n) (k:merkle_key) (c:bin_tree_dir)
   : option (base_key)
-  = let v = eac_value k il in
+  = let v = eac_merkle_value k il in
     if M.points_to_none c v
     then None
     else Some (M.pointed_key v c)
 
-let lemma_eac_value_is_stored_value
+let rec eac_ptrfn_empty_or_points_to_desc
   (#app #n:_)
   (il: eac_log app n)
-  (k:merkle_key)
-  (tid:nat{tid < n})
-  : Lemma (requires (store_contains (thread_store tid il) k))
-          (ensures (EACInStore? (eac_state_of_key k il) /\
-                    HI.eac_value (IntK k) il = HV.stored_value (thread_store tid il) k))
-  = eac_value_is_stored_value il (IntK k) tid
-
-let init_value = {left = Empty; right = Empty}
-
-let eac_value_init
-  (#app #n:_)
   (k: merkle_key)
+  (c: bin_tree_dir)
+  : Lemma (ensures (eac_ptrfn_aux il k c = None \/
+                    (let k' = Some?.v (eac_ptrfn_aux il k c) in
+                     is_desc k' (child c k))))
+          (decreases (length il))
+  = if length il = 0 then
+      eac_value_init (IntK k) il
+    else
+      let i = length il - 1  in
+      let il' = prefix il i in
+      let e = index il i in
+      eac_ptrfn_empty_or_points_to_desc il' k c;
+      eac_value_snoc (IntK k) il;
+      match e with
+      | RunApp _ _ _ -> only_data_keys_ref_runapp il i k
+      | _ -> ()
+
+let eac_ptrfn_base
+  (#app #n:_)
   (il: eac_log app n)
-  : Lemma (ensures (let es = eac_state_of_key k il in
-                    es = EACInit ==> eac_value k il = init_value))
-          [SMTPat (eac_value k il)]
-  = admit()
+  (k: bin_tree_node)
+  (c: bin_tree_dir)
+  : option(kd:bin_tree_node{is_desc kd (child c k)})
+  = if depth k >= key_size then None
+    else
+      let or = eac_ptrfn_aux il k c in
+      eac_ptrfn_empty_or_points_to_desc il k c;
+      if or = None then None
+      else Some (Some?.v or)
 
-(*
-let eac_value_unchanged_addb
+(* eac pointer function *)
+let eac_ptrfn
   (#app #n:_)
-  (il: eac_log app n{length il > 0})
-  (k: merkle_key)
-  : Lemma (requires (let i = length il - 1 in
-                     let e = index il i in
-                     AddB? e))
-          (ensures (let i = length il - 1 in
-                    let il' = prefix il i in
-                    eac_value k il = eac_value k il'))
-          [SMTPat (eac_value k il)]
-  = let i = length il - 1 in
-    let il' = prefix il i in
-    let e = index il i in
-    let es' = eac_state_of_key k il' in
-    let es = eac_state_of_key k il in
-    eac_state_snoc k il;
-
-    if e `refs_key` k then
-      admit()
-    else (
-      assert(es' = es);
-      match es' with
-      | EACInit -> ()
-      | EACInStore _ _ _ ->
-        admit()
-      | _ -> admit()
-    )
-let points_to_unchanged_addb
-  (#app #n:_)
-  (il: eac_log app n{length il > 0})
-  (k: merkle_key)
-  (c:bin_tree_dir)
-  : Lemma (requires (let i = length il - 1 in
-                     let e = index il i in
-                     AddB? e))
-          (ensures (let i = length il - 1 in
-                    let il' = prefix il i in
-                    ptrfn_aux il k c = ptrfn_aux il' k c))
-  = eac_value_unchanged_addb il k
-*)
+  (il: eac_log app n): ptrfn =
+  eac_ptrfn_base il
 
 (* the ancestor who holds the proof of the value of key k *)
 let proving_ancestor (#app #n:_) (il: eac_log app n) (k:base_key{k <> Root}):
@@ -113,7 +193,7 @@ let lemma_proving_ancestor_points_to_self (#app #n:_) (il: eac_log app n) (k:bas
   Lemma (requires (eac_state_of_key k il <> EACInit))
         (ensures (let pk = proving_ancestor il k in
                   let d = desc_dir k pk in
-                  let v = eac_value pk il in
+                  let v = eac_merkle_value pk il in
                   points_to v d k))
   = admit()
 
@@ -121,7 +201,7 @@ let lemma_proving_ancestor_points_to_self (#app #n:_) (il: eac_log app n) (k:bas
 let lemma_proving_ancestor_initial (#app #n:_) (il: eac_log app n) (k:base_key{k <> Root}):
   Lemma (requires (eac_state_of_key k il = EACInit))
         (ensures (let k' = proving_ancestor il k in
-                  let v' = eac_value k' il in
+                  let v' = eac_merkle_value k' il in
                   let c = desc_dir k k' in
                   points_to_none c v' \/
                   not (is_desc k (pointed_key v' c))))
@@ -133,7 +213,7 @@ let lemma_proving_ancestor_has_hash (#app #n:_) (il: eac_log app n) (gk:key app{
                    EACEvictedMerkle? (eac_state_of_key k il)))
         (ensures (let k = to_base_key gk in
                   let pk = proving_ancestor il k in
-                  let mv = eac_value pk il in
+                  let mv = eac_merkle_value pk il in
                   let c = desc_dir k pk in
                   let v = HI.eac_value gk il in
                   pointed_hash mv c = hashfn v))
@@ -175,7 +255,7 @@ let lemma_points_to_implies_proving_ancestor
   (k:base_key)
   (k':merkle_key)
   (d:bin_tree_dir):
-  Lemma (requires (let mv = eac_value k' il in
+  Lemma (requires (let mv = eac_merkle_value k' il in
                    points_to mv d k))
         (ensures (k <> Root /\ proving_ancestor il k = k'))
   = admit()
@@ -192,7 +272,7 @@ let lemma_init_ancestor_ancestor_of_proving
   Lemma (requires ((k' = Root \/ eac_state_of_key k' il <> EACInit) /\
                     k' <> proving_ancestor il k))
         (ensures (let d = desc_dir k k' in
-                  let mv = eac_value k' il in
+                  let mv = eac_merkle_value k' il in
                   let pk = proving_ancestor il k in
                   points_to_some mv d /\
                   is_desc pk (pointed_key mv d)))
@@ -201,9 +281,9 @@ let lemma_init_ancestor_ancestor_of_proving
 (* if a merkle value of key k points to a key kd in some direction d, then kd is a proper desc of
  * k in direction d *)
 let lemma_points_to_dir_correct (#app #n:_) (il: eac_log app n) (k:merkle_key) (d:bin_tree_dir):
-  Lemma (requires (let mv = eac_value k il in
+  Lemma (requires (let mv = eac_merkle_value k il in
                    points_to_some mv d))
-        (ensures (let mv = eac_value k il in
+        (ensures (let mv = eac_merkle_value k il in
                   let kd = pointed_key mv d in
                   is_proper_desc kd k /\
                   d = desc_dir kd k))
