generic/Zeta.Hash.fsti
@@ -7,3 +7,5 @@ let hash_size = 256
 
 (* hash value *)
 type hash_value = bv_t hash_size
+
+let zero: hash_value = zero_vec #hash_size
